Diverse improvements in utility module

code/experimental/utils/Hacl.Utils.Experimental.fst
@@ -17,9 +17,9 @@ module U8 = FStar.UInt8
 module U32 = FStar.UInt32
 module U64 = FStar.UInt64
 
-module S8 = Hacl.UInt8
-module S32 = Hacl.UInt32
-module S64 = Hacl.UInt64
+module H8 = Hacl.UInt8
+module H32 = Hacl.UInt32
+module H64 = Hacl.UInt64
 
 module Cast = Hacl.Cast
 
@@ -29,12 +29,12 @@ let uint8_t   = FStar.UInt8.t
 let uint32_t  = FStar.UInt32.t
 let uint64_t  = FStar.UInt64.t
 
-let suint8_t  = Hacl.UInt8.t
-let suint32_t = Hacl.UInt32.t
-let suint64_t = Hacl.UInt64.t
+let huint8_t  = Hacl.UInt8.t
+let huint32_t = Hacl.UInt32.t
+let huint64_t = Hacl.UInt64.t
 
-let suint32_p = Buffer.buffer suint32_t
-let suint8_p  = Buffer.buffer suint8_t
+let huint32_p = Buffer.buffer huint32_t
+let huint8_p  = Buffer.buffer huint8_t
 
 
 (* Definitions of aliases for functions *)
@@ -47,106 +47,97 @@ inline_for_extraction let u64_to_s64 = Cast.uint64_to_sint64
 
 
 [@"substitute"]
-val upd4: buf:suint32_p{length buf <= pow2 32} -> idx:uint32_t{U32.v idx + 3 < length buf /\ U32.v idx + 3 <= pow2 32} -> a:uint32_t -> b:uint32_t -> c:uint32_t -> d:uint32_t
-  -> Stack unit (requires (fun h -> live h buf))
-               (ensures  (fun h0 _ h1 -> live h1 buf /\ modifies_1 buf h0 h1))
-[@"substitute"]
-let upd4 buf idx a b c d =
-  buf.(idx +^ 0ul) <- u32_to_s32 a;
-  buf.(idx +^ 1ul) <- u32_to_s32 b;
-  buf.(idx +^ 2ul) <- u32_to_s32 c;
-  buf.(idx +^ 3ul) <- u32_to_s32 d
+val pupd_4: buf:huint32_p{length buf = 4} ->
+  v0:uint32_t -> v1:uint32_t -> v2:uint32_t -> v3:uint32_t ->
+  Stack unit (requires (fun h -> live h buf))
+               (ensures  (fun h0 _ h1 -> live h1 buf /\ modifies_1 buf h0 h1
+                         /\ (let s = Hacl.Spec.Endianness.reveal_h32s (as_seq h1 buf) in
+                           Seq.index s 0 == v0
+                         /\ Seq.index s 1 == v1
+                         /\ Seq.index s 2 == v2
+                         /\ Seq.index s 3 == v3)))
 
+[@"substitute"]
+let pupd_4 buf v0 v1 v2 v3 =
+  buf.(0ul) <- u32_to_s32 v0;
+  buf.(1ul) <- u32_to_s32 v1;
+  buf.(2ul) <- u32_to_s32 v2;
+  buf.(3ul) <- u32_to_s32 v3
+
+
+[@"substitute"]
+val upd_4: buf:huint32_p{length buf <= pow2 32} -> idx:uint32_t{U32.v idx + 3 < length buf /\ U32.v idx + 3 <= pow2 32} -> v0:uint32_t -> v1:uint32_t -> v2:uint32_t -> v3:uint32_t
+  -> Stack unit (requires (fun h -> live h buf))
+               (ensures  (fun h0 _ h1 -> live h1 buf /\ modifies_1 buf h0 h1
+                         (* /\ (let s = as_seq h1 buf in *)
+                         (* Seq.index s (U32.v idx + 0) == v0 /\ Seq.index s (U32.v idx + 1) == v1 /\ Seq.index s (U32.v idx + 2) == v2 /\ Seq.index s (U32.v idx + 3) == v3 )*)))
+[@"substitute"]
+let upd_4 buf idx v0 v1 v2 v3 =
+  buf.(idx +^ 0ul) <- u32_to_s32 v0;
+  buf.(idx +^ 1ul) <- u32_to_s32 v1;
+  buf.(idx +^ 2ul) <- u32_to_s32 v2;
+  buf.(idx +^ 3ul) <- u32_to_s32 v3
+
+
+[@"substitute"]
+val hupd_4: buf:huint32_p{length buf = 4} ->
+  v0:H32.t -> v1:H32.t -> v2:H32.t -> v3:H32.t ->
+  Stack unit (requires (fun h -> live h buf))
+             (ensures  (fun h0 _ h1 -> live h1 buf /\ modifies_1 buf h0 h1
+                         /\ (let s = as_seq h1 buf in
+                         Seq.index s 0 == v0 /\ Seq.index s 1 == v1 /\ Seq.index s 2 == v2 /\ Seq.index s 3 == v3)))
+
+[@"substitute"]
+let hupd_4 buf v0 v1 v2 v3 =
+  buf.(0ul) <- v0;
+  buf.(1ul) <- v1;
+  buf.(2ul) <- v2;
+  buf.(3ul) <- v3
+
+
+[@"substitute"]
+val hupd_8: buf:huint32_p{length buf = 8} ->
+  v0:H32.t -> v1:H32.t -> v2:H32.t -> v3:H32.t -> v4:H32.t -> v5:H32.t -> v6:H32.t -> v7:H32.t ->
+  Stack unit (requires (fun h -> live h buf))
+             (ensures  (fun h0 _ h1 -> live h1 buf /\ modifies_1 buf h0 h1
+                         /\ (let s = as_seq h1 buf in
+                         Seq.index s 0 == v0 /\ Seq.index s 1 == v1 /\ Seq.index s 2 == v2 /\ Seq.index s 3 == v3 /\
+                         Seq.index s 4 == v4 /\ Seq.index s 5 == v5 /\ Seq.index s 6 == v6 /\ Seq.index s 7 == v7)))
+
+[@"substitute"]
+let hupd_8 buf v0 v1 v2 v3 v4 v5 v6 v7 =
+  let p1 = Buffer.sub buf 0ul 4ul in
+  let p2 = Buffer.sub buf 4ul 4ul in
+  hupd_4 p1 v0 v1 v2 v3;
+  hupd_4 p2 v4 v5 v6 v7
+
+
+[@"substitute"]
+val pupd_8: buf:huint32_p{length buf = 8} ->
+  v0:uint32_t -> v1:uint32_t -> v2:uint32_t -> v3:uint32_t ->
+  v4:uint32_t -> v5:uint32_t -> v6:uint32_t -> v7:uint32_t ->
+  Stack unit (requires (fun h -> live h buf))
+             (ensures  (fun h0 _ h1 -> live h1 buf /\ modifies_1 buf h0 h1
+                       /\ (let s = Hacl.Spec.Endianness.reveal_h32s (as_seq h1 buf) in
+                         Seq.index s 0 == v0 /\ Seq.index s 1 == v1 /\ Seq.index s 2 == v2 /\ Seq.index s 3 == v3 /\
+                         Seq.index s 4 == v4 /\ Seq.index s 5 == v5 /\ Seq.index s 6 == v6 /\ Seq.index s 7 == v7)))
+[@"substitute"]
+let pupd_8 buf v0 v1 v2 v3 v4 v5 v6 v7 =
+  let h0 = u32_to_s32 v0 in
+  let h1 = u32_to_s32 v1 in
+  let h2 = u32_to_s32 v2 in
+  let h3 = u32_to_s32 v3 in
+  let h4 = u32_to_s32 v4 in
+  let h5 = u32_to_s32 v5 in
+  let h6 = u32_to_s32 v6 in
+  let h7 = u32_to_s32 v7 in
+  hupd_8 buf h0 h1 h2 h3 h4 h5 h6 h7
 
 
 (* Definition of the right rotation function for UInt32.t *)
 [@"substitute"]
-let rotate_right (a:suint32_t) (b:uint32_t{v b <= 32}) : Tot suint32_t =
-  S32.logor (S32.shift_right a b) (S32.shift_left a (U32.sub 32ul b))
-
-
-[@"substitute"]
-val be_bytes_of_sint32: b:suint8_p{length b >= 4} -> x:suint32_t
-  -> Stack unit
-          (requires (fun h -> live h b))
-          (ensures (fun h0 _ h1 -> live h1 b /\ modifies_1 b h0 h1))
-
-[@"substitute"]
-let be_bytes_of_sint32 output x =
- let b0 = sint32_to_sint8 (S32.logand (S32.shift_right x 24ul) (uint32_to_sint32 255ul)) in
- let b1 = sint32_to_sint8 (S32.logand (S32.shift_right x 16ul) (uint32_to_sint32 255ul)) in
- let b2 = sint32_to_sint8 (S32.logand (S32.shift_right x 8ul)  (uint32_to_sint32 255ul)) in
- let b3 = sint32_to_sint8 (S32.logand x (uint32_to_sint32 255ul)) in
- upd output 0ul b0;
- upd output 1ul b1;
- upd output 2ul b2;
- upd output 3ul b3
-
-
-[@"substitute"]
-val be_sint32_of_bytes: b:suint8_p{length b >= 4}
-  -> Stack suint32_t
-        (requires (fun h -> live h b))
-        (ensures (fun h0 r h1 -> live h1 b /\ modifies_1 b h0 h1))
-
-[@"substitute"]
-let be_sint32_of_bytes b =
-  let b0 = index b 0ul in
-  let b1 = index b 1ul in
-  let b2 = index b 2ul in
-  let b3 = index b 3ul in
-  let r =
-    S32.add_mod (S32.add_mod (S32.add_mod (sint8_to_sint32 b3)
-                                          (S32.op_Less_Less_Hat (sint8_to_sint32 b2) 8ul))
-	                          (S32.op_Less_Less_Hat (sint8_to_sint32 b1) 16ul))
-                (S32.op_Less_Less_Hat (sint8_to_sint32 b0) 24ul) in
-  r
-
-[@"substitute"]
-val be_bytes_of_sint64: b:suint8_p{length b >= 8} -> x:suint64_t
-  -> Stack unit
-        (requires (fun h -> live h b))
-        (ensures (fun h0 _ h1 -> live h1 b /\ modifies_1 b h0 h1))
-
-[@"substitute"]
-let be_bytes_of_sint64 output x =
- let b0 = sint64_to_sint8 (S64.logand (S64.shift_right x 56ul) (uint32_to_sint64 255ul)) in
- let b1 = sint64_to_sint8 (S64.logand (S64.shift_right x 48ul) (uint32_to_sint64 255ul)) in
- let b2 = sint64_to_sint8 (S64.logand (S64.shift_right x 40ul) (uint32_to_sint64 255ul)) in
- let b3 = sint64_to_sint8 (S64.logand (S64.shift_right x 32ul) (uint32_to_sint64 255ul)) in
- let b4 = sint64_to_sint8 (S64.logand (S64.shift_right x 24ul) (uint32_to_sint64 255ul)) in
- let b5 = sint64_to_sint8 (S64.logand (S64.shift_right x 16ul) (uint32_to_sint64 255ul)) in
- let b6 = sint64_to_sint8 (S64.logand (S64.shift_right x 8ul)  (uint32_to_sint64 255ul)) in
- let b7 = sint64_to_sint8 (S64.logand x (uint32_to_sint64 255ul)) in
- upd output 0ul b0;
- upd output 1ul b1;
- upd output 2ul b2;
- upd output 3ul b3;
- upd output 4ul b4;
- upd output 5ul b5;
- upd output 6ul b6;
- upd output 7ul b7
-
-
-val xor_bytes:
-  output :suint8_p ->
-  input  :suint8_p ->
-  len    :uint32_t{U32.v len <= length output /\ U32.v len <= length input} ->
-  Stack unit
-        (requires (fun h0 -> live h0 output /\ live h0 input))
-        (ensures  (fun h0 _ h1 -> live h1 output /\ modifies_1 output h0 h1))
-
-let rec xor_bytes output input len =
-  if U32.(len =^ 0ul) then ()
-  else
-    begin
-      let i    = U32.(len -^ 1ul) in
-      let in1i = Buffer.index input i in
-      let oi   = Buffer.index output i in
-      let oi   = S8.(in1i ^^ oi) in
-      output.(i) <- oi;
-      xor_bytes output input i
-    end
+let rotate_right (a:huint32_t) (b:uint32_t{v b <= 32}) : Tot huint32_t =
+  H32.logor (H32.shift_right a b) (H32.shift_left a (U32.sub 32ul b))
 
 
 val load32s_be:
@@ -189,3 +180,88 @@ let rec store32s_be buf_8 buf_32 len_32 =
       Hacl.Endianness.hstore32_be x_8 x_32;
       store32s_be buf_8 buf_32 FStar.UInt32.(len_32 -^ 1ul)
     end
+
+
+(* [@"substitute"] *)
+(* val be_bytes_of_sint32: b:huint8_p{length b >= 4} -> x:huint32_t *)
+(*   -> Stack unit *)
+(*           (requires (fun h -> live h b)) *)
+(*           (ensures (fun h0 _ h1 -> live h1 b /\ modifies_1 b h0 h1)) *)
+
+(* [@"substitute"] *)
+(* let be_bytes_of_sint32 output x = *)
+(*  let b0 = sint32_to_sint8 (H32.logand (H32.shift_right x 24ul) (uint32_to_sint32 255ul)) in *)
+(*  let b1 = sint32_to_sint8 (H32.logand (H32.shift_right x 16ul) (uint32_to_sint32 255ul)) in *)
+(*  let b2 = sint32_to_sint8 (H32.logand (H32.shift_right x 8ul)  (uint32_to_sint32 255ul)) in *)
+(*  let b3 = sint32_to_sint8 (H32.logand x (uint32_to_sint32 255ul)) in *)
+(*  upd output 0ul b0; *)
+(*  upd output 1ul b1; *)
+(*  upd output 2ul b2; *)
+(*  upd output 3ul b3 *)
+
+
+(* [@"substitute"] *)
+(* val be_sint32_of_bytes: b:huint8_p{length b >= 4} *)
+(*   -> Stack huint32_t *)
+(*         (requires (fun h -> live h b)) *)
+(*         (ensures (fun h0 r h1 -> live h1 b /\ modifies_1 b h0 h1)) *)
+
+(* [@"substitute"] *)
+(* let be_sint32_of_bytes b = *)
+(*   let b0 = index b 0ul in *)
+(*   let b1 = index b 1ul in *)
+(*   let b2 = index b 2ul in *)
+(*   let b3 = index b 3ul in *)
+(*   let r = *)
+(*     H32.add_mod (H32.add_mod (H32.add_mod (sint8_to_sint32 b3) *)
+(*                                           (H32.op_Less_Less_Hat (sint8_to_sint32 b2) 8ul)) *)
+(* 	                          (H32.op_Less_Less_Hat (sint8_to_sint32 b1) 16ul)) *)
+(*                 (H32.op_Less_Less_Hat (sint8_to_sint32 b0) 24ul) in *)
+(*   r *)
+
+
+(* [@"substitute"] *)
+(* val be_bytes_of_sint64: b:huint8_p{length b >= 8} -> x:huint64_t *)
+(*   -> Stack unit *)
+(*         (requires (fun h -> live h b)) *)
+(*         (ensures (fun h0 _ h1 -> live h1 b /\ modifies_1 b h0 h1)) *)
+
+(* [@"substitute"] *)
+(* let be_bytes_of_sint64 output x = *)
+(*  let b0 = sint64_to_sint8 (H64.logand (H64.shift_right x 56ul) (uint32_to_sint64 255ul)) in *)
+(*  let b1 = sint64_to_sint8 (H64.logand (H64.shift_right x 48ul) (uint32_to_sint64 255ul)) in *)
+(*  let b2 = sint64_to_sint8 (H64.logand (H64.shift_right x 40ul) (uint32_to_sint64 255ul)) in *)
+(*  let b3 = sint64_to_sint8 (H64.logand (H64.shift_right x 32ul) (uint32_to_sint64 255ul)) in *)
+(*  let b4 = sint64_to_sint8 (H64.logand (H64.shift_right x 24ul) (uint32_to_sint64 255ul)) in *)
+(*  let b5 = sint64_to_sint8 (H64.logand (H64.shift_right x 16ul) (uint32_to_sint64 255ul)) in *)
+(*  let b6 = sint64_to_sint8 (H64.logand (H64.shift_right x 8ul)  (uint32_to_sint64 255ul)) in *)
+(*  let b7 = sint64_to_sint8 (H64.logand x (uint32_to_sint64 255ul)) in *)
+(*  upd output 0ul b0; *)
+(*  upd output 1ul b1; *)
+(*  upd output 2ul b2; *)
+(*  upd output 3ul b3; *)
+(*  upd output 4ul b4; *)
+(*  upd output 5ul b5; *)
+(*  upd output 6ul b6; *)
+(*  upd output 7ul b7 *)
+
+
+(* val xor_bytes: *)
+(*   output :huint8_p -> *)
+(*   input  :huint8_p -> *)
+(*   len    :uint32_t{U32.v len <= length output /\ U32.v len <= length input} -> *)
+(*   Stack unit *)
+(*         (requires (fun h0 -> live h0 output /\ live h0 input)) *)
+(*         (ensures  (fun h0 _ h1 -> live h1 output /\ modifies_1 output h0 h1)) *)
+
+(* let rec xor_bytes output input len = *)
+(*   if U32.(len =^ 0ul) then () *)
+(*   else *)
+(*     begin *)
+(*       let i    = U32.(len -^ 1ul) in *)
+(*       let in1i = Buffer.index input i in *)
+(*       let oi   = Buffer.index output i in *)
+(*       let oi   = H8.(in1i ^^ oi) in *)
+(*       output.(i) <- oi; *)
+(*       xor_bytes output input i *)
+(*     end *)
